Split floyd/client_lemmas.v into two files, the new one is canon.v.
Added these definitions:
Definition temp (i: ident) (v: val) : environ -> Prop :=
   `(eq v) (eval_id i).
Definition var (i: ident) (t: type) (v: val) : environ -> Prop :=
   `(eq v) (eval_var i t).

and use them in many places in progs/verif_*.v.

Delete an unneeded "WITH" item in sha/spec_sha.v.

floyd/assert_lemmas.v
@@ -46,24 +46,6 @@ apply Share.contains_Rsh_e. apply top_correct'.
 Qed.
 Hint Resolve writable_share_top.
 
-Ltac safe_auto_with_closed := 
-   (* won't instantiate evars by accident *)
- match goal with |- ?A => 
-          solve [first [has_evar A | auto 50 with closed]]
- end.
-
-Lemma closed_env_set:
- forall {B} i v (P: environ -> B) rho, 
-     closed_wrt_vars (eq i) P -> 
-     P (env_set rho i v) = P rho.
-Proof.
- intros. hnf in H.
- symmetry; destruct rho; apply H.
- intros; simpl; destruct (ident_eq i i0). left; auto.
- right; rewrite Map.gso; auto.
-Qed.
-Hint Rewrite @closed_env_set using safe_auto_with_closed : norm.
-
 Lemma subst_derives:
   forall id e P Q, P |-- Q -> subst id e P |-- subst id e Q.
 Proof.
@@ -214,22 +196,6 @@ Lemma eval_expr_Etempvar' : forall i t, eval_id i = eval_expr (Etempvar i t).
 Proof. intros. symmetry; auto.
 Qed.
 Hint Resolve  eval_expr_Etempvar'.
-
-Lemma subst_eval_id_eq:
- forall id v, subst id v (eval_id id) = v.
-Proof. unfold subst, eval_id; intros. extensionality rho.
-    unfold force_val, env_set; simpl. rewrite Map.gss; auto.
-Qed.
-
-Lemma subst_eval_id_neq:
-  forall id v j, id<>j -> subst id v (eval_id j) = eval_id j.
-Proof.
-    unfold subst, eval_id; intros. extensionality rho.
-    unfold force_val, env_set; simpl. rewrite Map.gso; auto.
-Qed.
-
-Hint Rewrite subst_eval_id_eq : subst.
-Hint Rewrite subst_eval_id_neq using safe_auto_with_closed : subst.
 
 Hint Rewrite Int.add_zero  Int.add_zero_l Int.sub_zero_l : norm.
 
@@ -958,12 +924,6 @@ Lemma tc_andp_TT1:  forall e, tc_andp tc_TT e = e.
 Proof. intros; unfold tc_andp; reflexivity. Qed.
 Hint Rewrite tc_andp_TT1 tc_andp_TT2 : norm.
 
-Lemma prop_derives {A}{ND: NatDed A}: 
- forall (P Q: Prop), (P -> Q) -> prop P |-- prop Q.
-Proof.
-intros; apply prop_left; intro; apply prop_right; auto.
-Qed.
-
 Definition ptr_eq (v1 v2: val) : Prop :=
       match v1,v2 with
       | Vint n1, Vint n2 =>  Int.cmpu Ceq n1 n2 = true  /\ Int.cmpu Ceq n1 (Int.repr 0) = true
@@ -1323,129 +1283,3 @@ Proof.
 intros. destruct p; reflexivity.
 Qed.
 Hint Rewrite isptr_force_ptr' : norm.
-
-Fixpoint subst_eval_expr (j: ident) (v: environ -> val) (e: expr) : environ -> val :=
- match e with
- | Econst_int i ty => `(Vint i)
- | Econst_long i ty => `(Vlong i)
- | Econst_float f ty => `(Vfloat f)
- | Econst_single f ty => `(Vsingle f)
- | Etempvar id ty => if eqb_ident j id then v else eval_id id 
- | Eaddrof a ty => subst_eval_lvalue j v a 
- | Eunop op a ty =>  `(eval_unop op (typeof a)) (subst_eval_expr j v a) 
- | Ebinop op a1 a2 ty =>  
-                  `(eval_binop op (typeof a1) (typeof a2)) (subst_eval_expr j v a1) (subst_eval_expr j v a2)
- | Ecast a ty => `(eval_cast (typeof a) ty) (subst_eval_expr j v a)
- | Evar id ty => `(deref_noload ty) (eval_var id ty)
- | Ederef a ty => `(deref_noload ty) (`force_ptr (subst_eval_expr j v a))
- | Efield a i ty => `(deref_noload ty) (`(eval_field (typeof a) i) (subst_eval_lvalue j v a))
- end
-
- with subst_eval_lvalue (j: ident) (v: environ -> val) (e: expr) : environ -> val := 
- match e with 
- | Evar id ty => eval_var id ty
- | Ederef a ty => `force_ptr (subst_eval_expr j v a)
- | Efield a i ty => `(eval_field (typeof a) i) (subst_eval_lvalue j v a)
- | _  => `Vundef
- end.
-
-Lemma subst_eval_expr_eq:
-    forall j v e, subst j v (eval_expr e) = subst_eval_expr j v e
-with subst_eval_lvalue_eq: 
-    forall j v e, subst j v (eval_lvalue e) = subst_eval_lvalue j v e.
-Proof.
-intros j v; clear subst_eval_expr_eq; induction e; intros; simpl; try auto.
-unfold eqb_ident.
-unfold subst, eval_id, env_set, te_of. extensionality rho. 
-pose proof (Pos.eqb_spec j i).
-destruct H. subst. rewrite Map.gss. reflexivity.
-rewrite Map.gso; auto.
-rewrite <- IHe; clear IHe.
-unfold_lift.
-extensionality rho; unfold subst.
-reflexivity.
-unfold_lift.
-extensionality rho; unfold subst.
-rewrite <- IHe; reflexivity.
-unfold_lift.
-extensionality rho; unfold subst.
-rewrite <- IHe1, <- IHe2; reflexivity.
-unfold_lift.
-extensionality rho; unfold subst.
-rewrite <- IHe; reflexivity.
-unfold_lift.
-rewrite <- subst_eval_lvalue_eq.
-extensionality rho; unfold subst.
-f_equal. f_equal.
-
-intros j v; clear subst_eval_lvalue_eq; induction e; intros; simpl; try auto.
-unfold_lift.
-rewrite <- subst_eval_expr_eq.
-extensionality rho; unfold subst.
-f_equal.
-unfold_lift.
-extensionality rho; unfold subst.
-rewrite <- IHe.
-f_equal.
-Qed.
-
-Hint Rewrite subst_eval_expr_eq subst_eval_lvalue_eq : subst.
-
-
-Lemma closed_wrt_subst:
-  forall {A} id e (P: environ -> A), closed_wrt_vars (eq id) P -> subst id e P = P.
-Proof.
-intros.
-unfold subst, closed_wrt_vars in *.
-extensionality rho.
-symmetry.
-apply H.
-intros.
-destruct (eq_dec id i); auto.
-right.
-rewrite Map.gso; auto.
-Qed.
-
-Lemma closed_wrt_map_subst:
-   forall {A: Type} id e (Q: list (environ -> A)),
-         Forall (closed_wrt_vars (eq id)) Q ->
-         map (subst id e) Q = Q.
-Proof.
-induction Q; intros.
-simpl; auto.
-inv H.
-simpl; f_equal; auto.
-apply closed_wrt_subst; auto.
-Qed.
-Hint Rewrite @closed_wrt_map_subst using safe_auto_with_closed : subst.
-Hint Rewrite @closed_wrt_subst using safe_auto_with_closed : subst.
-
-Lemma closed_wrt_map_subst':
-   forall {A: Type} id e (Q: list (environ -> A)),
-         Forall (closed_wrt_vars (eq id)) Q ->
-         @map (LiftEnviron A) _ (subst id e) Q = Q.
-Proof.
-apply @closed_wrt_map_subst.
-Qed.
-
-Hint Rewrite @closed_wrt_map_subst' using safe_auto_with_closed : norm.
-Hint Rewrite @closed_wrt_map_subst' using safe_auto_with_closed : subst.
-Lemma closed_wrt_subst_eval_expr:
-  forall j v e, 
-   closed_wrt_vars (eq j) (eval_expr e) ->
-   subst_eval_expr j v e = eval_expr e.
-Proof.
-intros; rewrite <- subst_eval_expr_eq.
-apply closed_wrt_subst; auto.
-Qed.
-Lemma closed_wrt_subst_eval_lvalue:
-  forall j v e, 
-   closed_wrt_vars (eq j) (eval_lvalue e) ->
-   subst_eval_lvalue j v e = eval_lvalue e.
-Proof.
-intros; rewrite <- subst_eval_lvalue_eq.
-apply closed_wrt_subst; auto.
-Qed.
-Hint Rewrite closed_wrt_subst_eval_expr using solve [auto 50 with closed] : subst.
-Hint Rewrite closed_wrt_subst_eval_lvalue using solve [auto 50 with closed] : subst.
-
