floyd/base.v
@@ -7,4 +7,91 @@ Require veric.SeparationLogicSoundness.
 Export SeparationLogicSoundness.SoundSeparationLogic.CSL.
 Require Import veric.NullExtension.
 
+Local Open Scope logic.
 
+Lemma prop_and {A} {NA: NatDed A}: 
+    forall P Q: Prop, prop (P /\ Q) = (prop P && prop Q).
+Proof. intros. apply pred_ext. apply prop_left. intros [? ?]; normalize.
+   normalize.
+Qed.
+
+Hint Rewrite <- prop_and : gather_prop.
+
+Lemma gather_prop_left {A}{NA: NatDed A}:
+  forall P Q R,  !! P && (!! Q && R) = !!(P/\Q) && R.
+Proof. intros. rewrite <- andp_assoc. rewrite <- prop_and; auto.
+Qed.
+
+Lemma gather_prop_right {A}{NA: NatDed A}:
+  forall P Q R,  R && !! P && !! Q = !!(P/\Q) && R.
+Proof. intros. rewrite andp_assoc. rewrite andp_comm.  rewrite <- prop_and; auto.
+Qed.
+Hint Rewrite gather_prop_left gather_prop_right : gather_prop.
+
+Definition not_a_prop {A} (P: A) := True.
+
+Ltac not_a_prop := match goal with
+  | |- not_a_prop  (prop _) => fail 1 
+  | |- _ => apply I 
+end.
+
+Lemma flip_prop {A}{NA: NatDed A}: forall P Q, 
+      not_a_prop P -> (P&& !! Q = !! Q && P).
+Proof. intros. apply andp_comm. Qed.
+
+Hint Rewrite @flip_prop using not_a_prop : gather_prop.
+
+Lemma gather_prop3 {A}{NA: NatDed A}:
+  forall P Q R,  not_a_prop R -> not_a_prop Q -> R && (!! P && Q) = !!P && (R && Q).
+Proof. intros. rewrite andp_comm. rewrite andp_assoc.
+        rewrite (andp_comm Q); auto.
+Qed.
+
+Hint Rewrite @gather_prop3 using not_a_prop : gather_prop.
+
+
+Lemma gather_prop4 {A}{NA: NatDed A}:
+  forall P Q R,  not_a_prop R -> not_a_prop Q -> (!!P && R) && Q = !!P && (R && Q).
+Proof. intros. rewrite andp_assoc. auto. 
+Qed.
+Hint Rewrite @gather_prop4 using not_a_prop : gather_prop.
+
+Lemma gather_prop5 {A}{NA: NatDed A}:
+  forall P Q R,  not_a_prop R -> not_a_prop Q -> (R && !!P && Q) = !!P && (R && Q).
+Proof. intros. rewrite andp_assoc. rewrite andp_comm. rewrite andp_assoc.
+  f_equal; apply andp_comm.
+Qed.
+Hint Rewrite @gather_prop5 using not_a_prop : gather_prop.
+
+Hint Rewrite @sepcon_andp_prop @sepcon_andp_prop' : gather_prop.
+
+Hint Rewrite <- sepcon_assoc : gather_prop.
+
+Lemma prop_derives {A}{ND: NatDed A}: 
+ forall (P Q: Prop), (P -> Q) -> prop P |-- prop Q.
+Proof.
+intros; apply prop_left; intro; apply prop_right; auto.
+Qed.
+
+Lemma go_lower_lem1:
+  forall (P1 P: Prop) (QR PQR: mpred),
+      (P1 -> prop P && QR |-- PQR) ->
+      (prop (P1 /\ P ) && QR |-- PQR).
+Proof.
+ intros.
+ apply derives_extract_prop; intros [? ?].
+ apply derives_trans with (!!P && QR).
+ apply andp_right; auto. apply prop_right; auto.
+ apply H; auto.
+Qed.
+
+Lemma go_lower_lem1':
+  forall (P1 P2 P: Prop) (QR PQR: mpred),
+      (prop (P1 /\ (P2 /\ P)) && QR |-- PQR) ->
+      (prop ((P1 /\ P2) /\ P ) && QR |-- PQR).
+Proof.
+ intros.
+ eapply derives_trans;  [ | apply H].
+ apply andp_derives; auto.
+ apply prop_derives; intuition.
+Qed.
