floyd/canon.v
@@ -1,0 +1,1034 @@
+Require Import floyd.base.
+Local Open Scope logic.
+
+
+Definition PROPx (P: list Prop): forall (Q: environ->mpred), environ->mpred := 
+     andp (prop (fold_right and True P)).
+
+Notation "'PROP' ( x ; .. ; y )   z" := (PROPx (cons x%type .. (cons y%type nil) ..) z) (at level 10) : logic.
+Notation "'PROP' ()   z" :=   (PROPx nil z) (at level 10) : logic.
+Notation "'PROP' ( )   z" :=   (PROPx nil z) (at level 10) : logic.
+
+Definition LOCALx (Q: list (environ -> Prop)) : forall (R: environ->mpred), environ->mpred := 
+                 andp (local (fold_right (`and) (`True) Q)).
+
+Notation " 'LOCAL' ( )   z" := (LOCALx nil z)  (at level 9) : logic.
+Notation " 'LOCAL' ()   z" := (LOCALx nil z)  (at level 9) : logic.
+
+Notation " 'LOCAL' ( x ; .. ; y )   z" := (LOCALx (cons x%type .. (cons y%type nil) ..) z)
+         (at level 9) : logic.
+
+Definition SEPx: forall (R: list(environ->mpred)), environ->mpred := fold_right sepcon emp.
+Arguments SEPx R _ : simpl never.
+
+Notation " 'SEP' ( x ; .. ; y )" := (SEPx (cons x%logic .. (cons y%logic nil) ..))
+         (at level 8) : logic.
+
+Notation " 'SEP' ( ) " := (SEPx nil) (at level 8) : logic.
+Notation " 'SEP' () " := (SEPx nil) (at level 8) : logic.
+
+Lemma insert_local: forall Q1 P Q R,
+  local Q1 && (PROPx P (LOCALx Q (SEPx R))) = (PROPx P (LOCALx (Q1 :: Q) (SEPx R))).
+Proof.
+intros. extensionality rho.
+unfold PROPx, LOCALx, SEPx, local; super_unfold_lift. simpl.
+apply pred_ext; autorewrite with gather_prop; normalize;
+decompose [and] H; clear H.
+repeat apply andp_right; auto.
+apply prop_right; repeat split; auto.
+apply andp_right; auto.
+apply prop_right; repeat split; auto.
+Qed.
+Hint Rewrite insert_local:  norm.
+
+Lemma go_lower_lem20:
+  forall QR QR',
+    QR |-- QR' ->
+    PROPx nil QR |-- QR'.
+Proof. unfold PROPx; intros; intro rho; normalize. Qed.
+
+Ltac go_lowerx :=
+   unfold PROPx, LOCALx,SEPx, local, lift1; unfold_lift; intro rho; simpl;
+   repeat rewrite andp_assoc;
+   repeat ((simple apply go_lower_lem1 || apply derives_extract_prop || apply derives_extract_prop'); intro);
+   try apply prop_left;
+   repeat rewrite prop_true_andp by assumption;
+   try apply derives_refl.
+
+Lemma grab_tc_environ:
+  forall Delta P Q R S rho,
+    (tc_environ Delta rho -> (PROPx P (LOCALx Q R)) rho |-- S) ->
+    (PROPx P (LOCALx (tc_environ Delta :: Q) R)) rho |-- S.
+Proof.
+intros.
+unfold PROPx,LOCALx in *; simpl in *.
+normalize.
+change (!! tc_environ Delta rho && 
+              local  (fold_right `and `True Q) rho && R rho |-- S).
+normalize.
+rewrite (prop_true_andp _ _ H0) in H.
+auto.
+Qed.
+
+Fixpoint delete_nth {A} (n: nat) (xs: list A) {struct n} : list A :=
+ match n, xs with
+ | O, y::ys => ys
+ | S n', y::ys =>y :: delete_nth n' ys
+ | _ , _ => nil
+ end.
+
+Lemma grab_nth_LOCAL:
+   forall n P Q R,
+     (PROPx P (LOCALx Q (SEPx R))) = 
+     (PROPx P (LOCALx (nth n Q (lift0 True) :: delete_nth n Q) (SEPx R))).
+Proof.
+intros n P Q R.
+f_equal.
+unfold LOCALx, local; super_unfold_lift.
+f_equal.
+extensionality rho;  f_equal.
+revert Q; induction n; intros.
+destruct Q; simpl nth. unfold delete_nth.
+apply prop_ext; simpl; intuition.
+simpl. auto.
+destruct Q; simpl nth; unfold delete_nth; fold @delete_nth.
+apply prop_ext; simpl; intuition.
+simpl.
+apply prop_ext.
+rewrite (IHn Q).
+simpl.
+clear IHn.
+intuition.
+Qed.
+
+Lemma grab_nth_SEP:
+   forall n P Q R,
+    PROPx P (LOCALx Q (SEPx R)) = (PROPx P (LOCALx Q (SEPx (nth n R emp :: delete_nth n R)))).
+Proof.
+intros.
+f_equal. f_equal.
+extensionality rho; unfold SEPx.
+revert R; induction n; intros; destruct R.
+simpl. rewrite sepcon_emp; auto.
+simpl nth.
+unfold delete_nth.
+auto.
+simpl.
+rewrite sepcon_emp; auto.
+change (fold_right sepcon emp (m :: R) rho)
+  with (m rho * fold_right sepcon emp R rho).
+rewrite IHn.
+simpl.
+repeat rewrite <- sepcon_assoc.
+f_equal.
+apply sepcon_comm.
+Qed.
+
+Ltac find_in_list A L :=
+ match L with 
+  | A :: _ => constr:(O)
+  | _ :: ?Y => let n := find_in_list A Y in constr:(S n)
+  | nil => fail
+  end.
+
+Ltac length_of R :=
+ match R with
+  |  nil => constr:(O)
+  |  _:: ?R1 => let n := length_of R1 in constr:(S n)
+ end.
+
+Fixpoint insert {A} (n: nat) (x: A) (ys: list A) {struct n} : list A :=
+ match n with
+ | O => x::ys
+ | S n' => match ys with nil => x::ys | y::ys' => y::insert n' x ys' end
+end.
+
+(* Note: in the grab_indexes function,
+  it's important that the {struct} induction NOT be on xs, because
+  that list might not be concrete all the way to the end, where the ns list will be concrete.
+  Thus we do it this particular way.  *)
+Fixpoint  grab_indexes' {A} (ns: list (option nat)) (xs: list A) {struct ns} : list A * list A :=
+match ns, xs with
+| nil, xs => (nil, xs)
+| _, nil => (nil,nil)
+| Some n::ns', x::xs' => let (al,bl) := grab_indexes' ns' xs'
+                               in (insert n x al, bl)
+| None :: ns', x::xs' => let (al,bl) := grab_indexes' ns' xs'
+                                  in (al, x::bl)
+end.
+
+Fixpoint grab_calc' (k: Z) (z: nat) (ns: list (option nat)): list (option nat) :=
+match z, ns with
+| O, _::ns' => Some (nat_of_Z k) :: ns'
+| S z', None::ns' => None :: grab_calc' k z' ns'
+| S z', Some n :: ns => Some n :: grab_calc' (k-1) z' ns
+| O, nil => Some O :: nil
+| S z', nil => None :: grab_calc' k z' nil
+end.
+
+Fixpoint grab_calc (k: Z) (zs: list Z) (ns: list (option nat)) : list (option nat) :=
+match zs with
+| nil => ns
+| z::zs' => grab_calc (k+1) zs' (grab_calc' k (nat_of_Z z) ns)
+end.
+
+(* Eval compute in grab_calc 0 (3::1::5::nil) nil. *)
+
+(* Define app_alt, just like app, so we have better control
+  over which things get unfolded *)
+
+Definition app_alt {A: Type} :=
+fix app (l m : list A) : list A :=
+  match l with
+  | nil => m
+  | a :: l1 => a :: app l1 m
+  end.
+
+Definition grab_indexes {A} (ns: list Z) (xs: list A) : list A :=
+    let (al,bl) := grab_indexes' (grab_calc 0 ns nil) xs in app_alt al bl.
+
+(* TESTING 
+Variables (a b c d e f g h i j : assert).
+Eval compute in grab_indexes (1::4::6::nil) (a::b::c::d::e::f::g::h::i::j::nil).
+Eval compute in grab_indexes (1::6::4::nil) (a::b::c::d::e::f::g::h::i::j::nil).
+*) 
+
+Lemma fold_right_nil: forall {A B} (f: A -> B -> B) (z: B),
+   fold_right f z nil = z.
+Proof. reflexivity. Qed.
+Hint Rewrite @fold_right_nil : norm.
+Hint Rewrite @fold_right_nil : subst.
+
+Lemma fold_right_cons: forall {A B} (f: A -> B -> B) (z: B) x y,
+   fold_right f z (x::y) = f x (fold_right f z y).
+Proof. reflexivity. Qed.
+Hint Rewrite @fold_right_cons : norm.
+Hint Rewrite @fold_right_cons : subst.
+
+Lemma fold_right_sepcon_app {A} {NA: NatDed A} {SL: SepLog A}{CA: ClassicalSep A}:
+ forall P Q : list A, fold_right (@sepcon A NA SL) (@emp A NA SL) (P++Q) = 
+        fold_right sepcon emp P * fold_right sepcon emp Q.
+Proof.
+intros; induction P; simpl.
+rewrite emp_sepcon; auto.
+rewrite sepcon_assoc;
+f_equal; auto.
+Qed.
+
+Lemma grab_indexes_SEP : 
+  forall (ns: list Z) (xs: list(environ->mpred)),   SEPx xs = SEPx (grab_indexes ns xs).
+Proof.
+intros.
+unfold SEPx; extensionality rho.
+unfold grab_indexes. change @app_alt with  @app.
+forget (grab_calc 0 ns nil) as ks.
+revert xs; induction ks; intro.
+unfold grab_indexes'. simpl app. auto.
+destruct a.
+destruct xs. reflexivity.
+unfold grab_indexes'.
+fold @grab_indexes'.
+rewrite fold_right_cons.
+specialize (IHks xs).
+case_eq (grab_indexes' ks xs); intros.
+rewrite H in IHks.
+rewrite fold_right_app.
+transitivity (m rho * fold_right sepcon emp xs rho); try reflexivity.
+rewrite IHks.
+rewrite fold_right_app.
+forget (fold_right sepcon emp l0) as P.
+transitivity (fold_right sepcon P (m::l) rho). reflexivity.
+clear.
+revert l; induction n; intro l. reflexivity.
+simpl. destruct l. simpl. auto.
+simpl. rewrite <- sepcon_assoc. rewrite (sepcon_comm (m rho)).
+rewrite sepcon_assoc. f_equal.
+specialize (IHn l). simpl in IHn.
+auto.
+destruct xs. reflexivity.
+unfold grab_indexes'.
+fold @grab_indexes'.
+rewrite fold_right_cons.
+specialize (IHks xs).
+case_eq (grab_indexes' ks xs); intros.
+rewrite H in IHks.
+simpl.
+simpl in IHks; rewrite IHks.
+clear.
+induction l; simpl; auto.
+rewrite <- IHl.
+clear IHl.
+repeat rewrite <- sepcon_assoc.
+f_equal.
+rewrite sepcon_comm; auto.
+Qed.
+
+(* The simpl_nat_of_P tactic is a complete hack,
+  needed for compatibility between Coq 8.3/8.4,
+  because the name of the thing to unfold varies
+  between the two versions *)
+Ltac simpl_nat_of_P :=
+match goal with |- context [nat_of_P ?n] =>
+  match n with xI _ => idtac | xO _ => idtac | xH => idtac | _ => fail end;
+  let N := fresh "N" in
+  set (N:= nat_of_P n);
+  compute in N;
+  unfold N; clear N
+end.
+
+Ltac grab_indexes_SEP ns :=
+  rewrite (grab_indexes_SEP ns); 
+    unfold grab_indexes; simpl grab_calc; 
+   unfold grab_indexes', insert; 
+   repeat simpl_nat_of_P; cbv beta iota;
+   unfold app_alt; fold @app_alt.
+
+Tactic Notation "focus_SEP" constr(a) := grab_indexes_SEP (a::nil).
+Tactic Notation "focus_SEP" constr(a) constr(b) := grab_indexes_SEP (a::b::nil).
+Tactic Notation "focus_SEP" constr(a) constr(b) constr(c) := 
+   grab_indexes_SEP (a::b::c::nil).
+Tactic Notation "focus_SEP" constr(a) constr(b) constr(c) constr(d) := 
+   grab_indexes_SEP (a::b::c::d::nil).
+
+(* TESTING 
+Variables (a b c d e f g h i j : assert).
+Goal (SEP (a;b;c;d;e;f;g;h;i;j) = SEP (b;d;a;c;e;f;g;h;i;j)).
+focus_SEP 1 3.
+auto.
+Qed.
+Goal (SEP (a;b;c;d;e;f;g;h;i;j) = SEP (d;b;a;c;e;f;g;h;i;j)).
+focus_SEP 3 1. 
+auto.
+Qed.
+
+*)
+
+Lemma semax_post0:
+ forall (R': ret_assert) Espec Delta (R: ret_assert) P c,
+   (R' |-- R) ->
+   @semax Espec Delta P c R' ->  @semax Espec Delta P c R.
+Proof.
+intros; eapply semax_pre_post; try eassumption.
+apply andp_left2; auto.
+intros. apply andp_left2; auto.
+apply H.
+Qed.
+
+Lemma local_unfold: forall P rho, local P rho = !! (P rho).
+Proof. reflexivity. Qed.
+Hint Rewrite local_unfold : norm.
+
+Lemma lower_sepcon:
+  forall P Q rho, @sepcon (environ->mpred) _ _ P Q rho = sepcon (P rho) (Q rho).
+Proof. reflexivity. Qed.
+Lemma lower_andp:
+  forall P Q rho, @andp (environ->mpred) _ P Q rho = andp (P rho) (Q rho).
+Proof. reflexivity. Qed.
+Hint Rewrite lower_sepcon lower_andp : norm.
+
+Lemma lift_prop_unfold: 
+   forall P z,  @prop (environ->mpred) _ P z = @prop mpred Nveric P.
+Proof.  reflexivity. Qed.
+Hint Rewrite lift_prop_unfold: norm.
+
+Lemma andp_unfold: forall (P Q: environ->mpred) rho,
+  @andp (environ->mpred) _ P Q rho = @andp mpred Nveric (P rho) (Q rho).
+Proof. reflexivity. Qed.
+Hint Rewrite andp_unfold: norm.
+
+Lemma exp_unfold : forall A P rho,
+ @exp (environ->mpred) _ A P rho = @exp mpred Nveric A (fun x => P x rho).
+Proof.
+intros. reflexivity. 
+Qed.
+Hint Rewrite exp_unfold: norm.
+
+Lemma semax_frame_PQR:
+  forall Espec Delta R1 R2 P Q P' Q' R1' c,
+     closed_wrt_modvars c (SEPx R2) ->
+     @semax Espec Delta (PROPx P (LOCALx Q (SEPx R1))) c 
+                     (normal_ret_assert (PROPx P' (LOCALx Q' (SEPx R1')))) ->
+     @semax Espec Delta (PROPx P (LOCALx Q (SEPx (R1++R2)))) c 
+                     (normal_ret_assert (PROPx P' (LOCALx Q' (SEPx (R1'++R2))))).
+Proof.
+intros.
+replace (PROPx P (LOCALx Q (SEPx (R1 ++ R2))))
+   with (PROPx P (LOCALx Q (SEPx (R1))) * SEPx R2).
+eapply semax_post0; [ | apply semax_frame; eassumption].
+intros ek vl rho.
+unfold frame_ret_assert, normal_ret_assert; 
+ destruct ek; simpl; normalize; try congruence.
+match goal with |- ?A |-- ?B => replace B with A; auto end.
+f_equal.
+unfold PROPx,LOCALx,SEPx.
+normalize.
+rewrite fold_right_sepcon_app; normalize.
+extensionality rho; unfold PROPx,LOCALx,SEPx.
+rewrite fold_right_sepcon_app; normalize.
+Qed.
+
+Lemma derives_frame_PQR:
+  forall R1 R2 P Q P' Q' R1',
+  PROPx P (LOCALx Q (SEPx R1)) |-- PROPx P' (LOCALx Q' (SEPx R1')) ->
+  PROPx P (LOCALx Q (SEPx (R1++R2))) |-- PROPx P' (LOCALx Q' (SEPx (R1'++R2))).
+Proof.
+intros.
+eapply derives_trans; [ | eapply derives_trans].
+2: apply sepcon_derives; [ apply H | apply (derives_refl  (fold_right sepcon emp R2))].
+clear H.
+unfold PROPx, LOCALx, SEPx, local; super_unfold_lift; intros.
+rewrite fold_right_sepcon_app.
+intro rho; simpl; normalize.
+unfold PROPx, LOCALx, SEPx, local; super_unfold_lift; intros.
+rewrite fold_right_sepcon_app.
+intro rho; simpl; normalize.
+Qed.
+
+Ltac frame_SEP' L :=
+  grab_indexes_SEP L;
+ match goal with
+ | |- @semax _ _ (PROPx _ (LOCALx _ (SEPx ?R))) _ _ => 
+  rewrite <- (firstn_skipn (length L) R); 
+    simpl length; unfold firstn, skipn;
+    eapply semax_frame_PQR;
+      [ unfold closed_wrt_modvars;  auto 50 with closed
+     | ]
+ | |- (PROPx _ (LOCALx _ (SEPx ?R))) |-- _ => 
+  rewrite <- (firstn_skipn (length L) R); 
+    simpl length; unfold firstn, skipn;
+    apply derives_frame_PQR
+end.
+
+Tactic Notation "frame_SEP" constr(a) := frame_SEP' (a::nil).
+Tactic Notation "frame_SEP" constr(a) constr(b) := frame_SEP' (a::b::nil).
+Tactic Notation "frame_SEP" constr(a) constr(b) constr(c) := 
+   frame_SEP' (a::b::c::nil).
+Tactic Notation "frame_SEP" constr(a) constr(b) constr(c) constr(d) := 
+   frame_SEP' (a::b::c::d::nil).
+
+Lemma gather_SEP:
+  forall R1 R2, 
+    SEPx (R1 ++ R2) = SEPx (fold_right sepcon emp R1 :: R2).
+Proof. 
+intros.
+unfold SEPx.
+extensionality rho.
+induction R1; simpl. rewrite emp_sepcon; auto.
+rewrite sepcon_assoc; f_equal; auto.
+Qed.
+
+Ltac gather_SEP' L :=
+   grab_indexes_SEP L;
+ match goal with |- context [SEPx ?R] => 
+    let r := fresh "R" in 
+    set (r := (SEPx R));
+    revert r;
+     rewrite <- (firstn_skipn (length L) R);
+      unfold length at 1 2;
+      unfold firstn at 1; unfold skipn at 1;
+      rewrite gather_SEP;
+   unfold fold_right at 1; try  rewrite sepcon_emp;
+   intro r; unfold r; clear r
+ end.
+
+Tactic Notation "gather_SEP" constr(a) := gather_SEP' (a::nil).
+Tactic Notation "gather_SEP" constr(a) constr(b) := gather_SEP' (a::b::nil).
+Tactic Notation "gather_SEP" constr(a) constr(b) constr(c) := 
+   gather_SEP' (a::b::c::nil).
+Tactic Notation "gather_SEP" constr(a) constr(b) constr(c) constr(d) := 
+   gather_SEP' (a::b::c::d::nil).
+
+
+Fixpoint replace_nth {A} (n: nat) (al: list A) (x: A) {struct n}: list A :=
+ match n, al with
+ | O , a::al => x::al
+ | S n', a::al' => a :: replace_nth n' al' x
+ | _, nil => nil
+ end.
+
+Fixpoint my_nth{A} (n: nat) (al: list A) (default: A) {struct n} : A :=
+  (* just like nth; make a new copy, for better control of unfolding *)
+match n, al with
+| O, a::al' => a
+| S n', a::al' => my_nth n' al' default
+| _, nil => default
+end.
+
+Lemma semax_pre_simple:
+ forall P' Espec Delta P c R,
+     (local (tc_environ Delta) && P |-- P') ->
+     @semax Espec Delta P' c R  -> @semax Espec Delta P c R.
+Proof.
+intros; eapply semax_pre_post; eauto.
+intros; apply andp_left2; auto.
+Qed.
+
+Lemma semax_pre0:
+ forall P' Espec Delta P c R,
+     P |-- P' ->
+     @semax Espec Delta P' c R  -> 
+     @semax Espec Delta P c R.
+Proof.
+intros.
+eapply semax_pre_simple; try apply H0.
+ apply andp_left2; auto.
+Qed.
+
+Lemma semax_pre:
+ forall P' Espec Delta P1 P2 P3 c R,
+     (PROPx P1 (LOCALx (tc_environ Delta :: P2) (SEPx P3))) |-- P' ->
+     @semax Espec Delta P' c R  -> 
+     @semax Espec Delta (PROPx P1 (LOCALx P2 (SEPx P3))) c R.
+Proof.
+intros.
+eapply semax_pre_simple; try apply H0.
+ rewrite insert_local. auto.
+Qed.
+
+Lemma replace_SEP':
+ forall n R' Espec Delta P Q Rs c Post,
+ (PROPx P (LOCALx (tc_environ Delta :: Q) (SEPx (my_nth n Rs TT ::  nil)))) |-- R' ->
+ @semax Espec Delta (PROPx P (LOCALx Q (SEPx (replace_nth n Rs R')))) c Post ->
+ @semax Espec Delta (PROPx P (LOCALx Q (SEPx Rs))) c Post.
+Proof.
+intros.
+eapply semax_pre; [ | apply H0].
+clear - H.
+unfold PROPx, LOCALx, SEPx in *; intro rho; specialize (H rho).
+unfold local, lift1 in *.
+simpl in *; unfold_lift; unfold_lift in H.
+normalize.
+rewrite prop_true_andp in H by auto.
+rewrite prop_true_andp in H by auto.
+destruct H1; normalize.
+clear - H.
+rewrite sepcon_emp in H.
+
+revert Rs H; induction n; destruct Rs; simpl ; intros; auto;
+apply sepcon_derives; auto.
+Qed.
+
+Ltac replace_SEP n R :=
+  apply (replace_SEP' (nat_of_Z n) R);
+  unfold my_nth,replace_nth; simpl nat_of_Z;
+   repeat simpl_nat_of_P; cbv beta iota; cbv beta iota.
+
+Ltac replace_in_pre S S' :=
+ match goal with |- @semax _ _ ?P _ _ =>
+  match P with context C[S] =>
+     let P' := context C[S'] in 
+      apply semax_pre with P'; [ | ]
+  end
+ end.
+
+Lemma semax_extract_PROP_True:
+  forall Espec Delta (PP: Prop) P QR c Post,
+        PP ->
+        @semax Espec Delta (PROPx P QR) c Post -> 
+       @semax Espec Delta (PROPx (PP::P) QR) c Post.
+Proof.
+intros.
+apply semax_pre_simple with (PROPx P QR); auto.
+clear.
+intro rho; unfold PROPx in *; simpl. normalize.
+destruct H; normalize.
+Qed.
+
+Lemma semax_extract_PROP:
+  forall Espec Delta (PP: Prop) P QR c Post,
+       (PP -> @semax Espec Delta (PROPx P QR) c Post) -> 
+       @semax Espec Delta (PROPx (PP::P) QR) c Post.
+Proof.
+intros.
+apply semax_pre_simple with (!!PP && PROPx P QR).
+intro rho; unfold PROPx in *; simpl; normalize.
+destruct H0; normalize.
+apply semax_extract_prop.
+auto.
+Qed.
+
+Lemma PROP_later_derives:
+ forall P QR QR', QR |-- |>QR' ->
+    PROPx P QR |-- |> PROPx P QR'.
+Proof.
+intros.
+unfold PROPx.
+normalize.
+Qed.
+
+Lemma LOCAL_later_derives:
+ forall Q R R', R |-- |>R' -> LOCALx Q R |-- |> LOCALx Q R'.
+Proof.
+unfold LOCALx; intros; normalize.
+rewrite later_andp.
+apply andp_derives; auto.
+apply now_later.
+Qed.
+
+Lemma SEP_later_derives:
+  forall P Q P' Q', 
+      P |-- |> P' ->
+      SEPx Q |-- |> SEPx Q' ->
+      SEPx (P::Q) |-- |> SEPx (P'::Q').
+Proof.
+unfold SEPx.
+intros.
+intro rho.
+specialize (H0 rho).
+intros; normalize.
+simpl.
+rewrite later_sepcon.
+apply sepcon_derives; auto.
+apply H.
+Qed.
+Hint Resolve PROP_later_derives LOCAL_later_derives SEP_later_derives : derives.
+
+Lemma local_lift0: forall P, local (lift0 P) = prop P.
+Proof.
+intros. extensionality rho. reflexivity.
+Qed.
+Hint Rewrite @local_lift0: norm.
+
+Lemma move_prop_from_LOCAL:
+  forall P1 P Q R, PROPx P (LOCALx (lift0 P1::Q) R) = PROPx (P1::P) (LOCALx Q R).
+Proof.
+ intros.
+ extensionality rho.
+ unfold PROPx, LOCALx, local, lift0, lift1.
+ unfold_lift.
+ simpl.
+ apply pred_ext; normalize.
+ destruct H0. repeat rewrite prop_true_andp by auto; auto.
+ destruct H.  repeat rewrite prop_true_andp by auto; auto.
+Qed.
+
+Ltac extract_prop_from_LOCAL :=
+ match goal with |- @semax _ _ (PROPx _ (LOCALx ?Q _)) _ _ =>
+   match Q with 
+    | context [ lift0 ?z :: _ ] =>
+        let n := find_in_list (lift0 z) Q
+         in rewrite (grab_nth_LOCAL n); 
+             unfold nth, delete_nth; 
+             rewrite move_prop_from_LOCAL
+   | context [@liftx (LiftEnviron Prop) ?z :: _ ] =>
+       let n := find_in_list (@liftx (LiftEnviron Prop) z) Q
+         in rewrite (grab_nth_LOCAL n); 
+             change (@liftx (LiftEnviron Prop) z) with (@lift0 Prop z);
+             unfold nth, delete_nth; 
+             rewrite move_prop_from_LOCAL
+  end
+end.
+Lemma semax_post:
+ forall (R': ret_assert) Espec Delta (R: ret_assert) P c,
+   (forall ek vl, local (tc_environ (exit_tycon c Delta ek)) &&  R' ek vl |-- R ek vl) ->
+   @semax Espec Delta P c R' ->  @semax Espec Delta P c R.
+Proof.
+intros; eapply semax_pre_post; try eassumption.
+apply andp_left2; auto.
+Qed.
+
+Lemma semax_post_flipped:
+  forall (R' : ret_assert) Espec (Delta : tycontext) (R : ret_assert)
+         (P : environ->mpred) (c : statement),
+        @semax Espec Delta P c R' -> 
+       (forall (ek : exitkind) (vl : option val),
+        local (tc_environ (exit_tycon c Delta ek)) && R' ek vl |-- R ek vl) ->
+       @semax Espec Delta P c R.
+Proof. intros; eapply semax_post; eassumption. Qed.
+
+
+Lemma semax_post': forall R' Espec Delta R P c,
+           R' |-- R ->
+      @semax Espec Delta P c (normal_ret_assert R') ->
+      @semax Espec Delta P c (normal_ret_assert R).
+Proof. intros. eapply semax_post; eauto. intros. apply andp_left2.
+  intro rho; unfold normal_ret_assert; normalize.
+Qed.
+
+Lemma extract_exists_pre:
+      forall
+        (A : Type) (P : A -> environ->mpred) (c : Clight.statement)
+         Espec Delta  (R : ret_assert),
+       (forall x : A, @semax Espec Delta (P x) c R) ->
+       @semax Espec Delta (exp (fun x => P x)) c R.
+Proof.
+intros.
+apply semax_post with (existential_ret_assert (fun _:A => R)).
+intros ek vl.
+unfold existential_ret_assert.
+apply andp_left2.
+apply exp_left; auto.
+apply extract_exists; auto.
+Qed.
+
+Lemma extract_exists_post:
+  forall {Espec: OracleKind} {A: Type} (x: A) Delta 
+       (P: environ -> mpred) c (R: A -> environ -> mpred),
+  semax Delta P c (normal_ret_assert (R x)) ->
+  semax Delta P c (normal_ret_assert (exp R)).
+Proof.
+intros.
+eapply semax_pre_post; try apply H.
+apply andp_left2; auto.
+intros ek vl rho.
+unfold local, lift1, existential_ret_assert.
+simpl.
+apply andp_left2.
+unfold normal_ret_assert.
+normalize.
+apply exp_right with x; normalize.
+Qed.
+
+Ltac repeat_extract_exists_pre :=
+   first [(apply extract_exists_pre;
+             let x := fresh "x" in intro x; normalize;
+                repeat_extract_exists_pre;
+                revert x)
+           | autorewrite with canon
+          ].
+             
+Lemma extract_exists_in_SEP:
+  forall {A} (R1: A -> environ->mpred) P Q R,   
+    PROPx P (LOCALx Q (SEPx (exp R1 :: R))) = 
+    EX x:A, PROPx P (LOCALx Q (SEPx (R1 x::R))).
+Proof.
+intros.
+extensionality rho.
+unfold PROPx, LOCALx, SEPx; simpl.
+normalize.
+Qed.
+
+Ltac extract_exists_in_SEP :=
+ match goal with |- @semax _ _ (PROPx _ (LOCALx _ (SEPx ?R))) _ _ =>
+   match R with context [ exp ?z :: _] =>
+        let n := find_in_list (exp z) R 
+         in rewrite (grab_nth_SEP n); unfold nth, delete_nth; rewrite extract_exists_in_SEP;
+             repeat_extract_exists_pre
+  end
+end.
+
+Lemma flatten_sepcon_in_SEP:
+  forall P Q R1 R2 R, 
+           PROPx P (LOCALx Q (SEPx ((R1*R2) :: R))) = 
+           PROPx P (LOCALx Q (SEPx (R1 :: R2 :: R))).
+Proof.
+intros.
+f_equal. f_equal. extensionality rho.
+unfold SEPx.
+simpl. rewrite sepcon_assoc. auto.
+Qed.
+
+Ltac flatten_sepcon_in_SEP :=
+  match goal with |- @semax _ _ (PROPx _ (LOCALx _ (SEPx ?R))) _ _ =>
+   match R with context [ (sepcon ?x  ?y) :: ?R'] =>
+  let n := length_of R in let n' := length_of R' in 
+         rewrite (grab_nth_SEP (n-S n')); simpl minus; unfold nth, delete_nth; 
+         rewrite flatten_sepcon_in_SEP
+end
+end.
+Lemma semax_ff:
+  forall Espec Delta c R,  
+   @semax Espec Delta FF c R.
+Proof.
+intros.
+apply semax_pre_post with (FF && FF) R.
+apply andp_left2. apply andp_right; auto.
+intros; apply andp_left2; auto.
+apply semax_extract_prop. intros; contradiction.
+Qed.
+
+Lemma sequential:
+  forall Espec Delta P c Q,
+        @semax Espec Delta P c (normal_ret_assert (Q EK_normal None)) ->
+          @semax Espec Delta P c Q.
+intros. eapply semax_post; eauto.
+ intros. intro rho. unfold local,lift1; simpl.
+ unfold normal_ret_assert; simpl.
+ normalize.
+Qed.
+
+Lemma sequential': 
+    forall Q Espec Delta P c R,
+               @semax Espec Delta P c (normal_ret_assert Q) -> 
+               @semax Espec Delta P c (overridePost Q R).
+Proof.
+intros.
+apply semax_post with (normal_ret_assert Q); auto.
+intros.
+unfold normal_ret_assert, overridePost.
+normalize.
+rewrite if_true; auto.
+apply andp_left2; auto.
+Qed.
+
+Lemma extract_prop_in_SEP:
+  forall n P1 Rn P Q R, 
+   nth n R emp = prop P1 && Rn -> 
+   PROPx P (LOCALx Q (SEPx R)) = PROPx (P1::P) (LOCALx Q (SEPx (replace_nth n R Rn))).
+Proof.
+intros.
+extensionality rho.
+unfold PROPx,LOCALx,SEPx,local,lift1.
+simpl.
+apply pred_ext; normalize.
+* match goal with |- _ |-- !! ?PP && _ => replace PP with P1
+   by (apply prop_ext; intuition)
+  end.
+  rewrite (prop_true_andp _ _ H1).
+ clear H1 Q H0 P.
+  clear - H.
+  revert R H; induction n; destruct R; simpl; intros.
+  apply andp_right; auto.
+  apply equal_f with rho in H.
+  rewrite H; apply andp_left1; auto.
+  rewrite H.
+  normalize.
+  apply andp_right; auto.
+  apply equal_f with rho in H.
+  rewrite H; apply andp_left1; auto.
+  rewrite <- sepcon_andp_prop.
+  apply sepcon_derives; auto.
+*
+  destruct H0; repeat rewrite prop_true_andp by auto.
+ clear - H H0.
+  revert R H; induction n; destruct R; simpl; intros; auto. 
+  subst m. rewrite prop_true_andp; auto.
+  apply sepcon_derives; auto.
+Qed.
+
+Lemma insert_SEP: 
+ forall R1 P Q R, R1 * PROPx P (LOCALx Q (SEPx R)) = PROPx P (LOCALx Q (SEPx (R1::R))).
+Proof.
+intros. 
+unfold PROPx,LOCALx,SEPx,local,lift1.
+extensionality rho; simpl.
+repeat rewrite sepcon_andp_prop. f_equal; auto.
+Qed.
+
+Lemma delete_emp_in_SEP:
+  forall n (R: list (environ->mpred)), 
+    nth_error R n = Some emp ->
+    SEPx R = SEPx (firstn n R ++ list_drop (S n) R).
+Proof.
+intros.
+unfold SEPx; extensionality rho.
+revert R H; induction n; destruct R; simpl; intros; auto.
+inv H. rewrite emp_sepcon; auto.
+f_equal; auto.
+etransitivity.
+apply IHn; auto.
+reflexivity.
+Qed.
+
+Ltac delete_emp_in_SEP :=
+ change (@liftx (LiftEnviron mpred) (@emp mpred _ _)) with 
+       (@emp (environ->mpred) _ _); 
+ repeat  
+ match goal with |- context [SEPx ?R] =>
+   match R with context [emp:: ?R'] =>
+     rewrite (delete_emp_in_SEP (length R - S (length R')) R) by reflexivity;
+     simpl length; simpl minus; unfold firstn, app, list_drop; fold app
+   end
+ end.
+
+Lemma extract_local_in_SEP :
+  forall n Q1 Rn P Q R, 
+   nth_error R n = Some (local Q1 && Rn) -> 
+   PROPx P (LOCALx Q (SEPx R)) = PROPx P (LOCALx (Q1::Q) (SEPx (replace_nth n R Rn))).
+Proof.
+intros.
+f_equal.
+extensionality rho.
+unfold PROPx,LOCALx,SEPx,local,lift1 in *.
+unfold_lift; simpl in *.
+revert R H; induction n; destruct R; simpl; intros;
+ inv H.
+apply pred_ext; subst; normalize.
+rewrite prop_true_andp by auto.
+auto.
+destruct H; normalize.
+specialize (IHn R).
+do 2 rewrite <- sepcon_andp_prop.
+rewrite IHn.
+auto.
+auto.
+Qed.
+
+Ltac move_local_from_SEP :=
+match goal with |- context [PROPx _ (LOCALx _ (SEPx ?R))] =>
+  match R with context [(local ?P1 && ?Rn) :: ?R'] =>
+  let n := length_of R in let n' := length_of R' in 
+   rewrite (extract_local_in_SEP (n-S n')%nat P1 Rn) by reflexivity;
+    simpl minus; unfold replace_nth 
+ end
+end.
+
+Ltac move_from_SEP :=
+  (* combines extract_exists_in_SEP, move_prop_from_SEP, move_local_from_SEP, 
+                  flatten_sepcon_in_SEP *)
+match goal with |- context [PROPx _ (LOCALx _ (SEPx ?R))] =>
+  match R with 
+  | context [(local ?P1 && ?Rn) :: ?R'] =>
+      let n := length_of R in let n' := length_of R' in 
+       rewrite (extract_local_in_SEP (n-S n')%nat P1 Rn) by reflexivity;
+        simpl minus; unfold replace_nth 
+  | context [(prop ?P1 && ?Rn) :: ?R'] =>
+      let n := length_of R in let n' := length_of R' in 
+        rewrite (extract_prop_in_SEP (n-S n')%nat P1 Rn) by reflexivity;
+        simpl minus; unfold replace_nth (*;
+        try (apply semax_extract_PROP; intro)*)
+  | context [ exp ?z :: _] =>
+        let n := find_in_list (exp z) R 
+         in rewrite (grab_nth_SEP n); unfold nth, delete_nth; rewrite extract_exists_in_SEP;
+             repeat_extract_exists_pre
+  | context [ (sepcon ?x  ?y) :: ?R'] =>
+        let n := length_of R in let n' := length_of R' in 
+         rewrite (grab_nth_SEP (n-S n')); simpl minus; unfold nth, delete_nth; 
+         rewrite flatten_sepcon_in_SEP
+ end
+end.
+
+
+Lemma move_local_from_SEP':
+  forall P1 R1 P Q R, 
+      PROPx P (LOCALx Q (SEPx ((local P1&&R1) :: R))) = PROPx P (LOCALx (P1::Q) (SEPx (R1::R))).
+Proof.
+ intros.
+ extensionality rho.
+ unfold PROPx, LOCALx, SEPx, local, lift1; unfold_lift.
+ normalize.
+ apply pred_ext; normalize.
+ rewrite prop_true_andp by auto. auto.
+ destruct H0; normalize.
+Qed.
+
+Lemma nth_error_local:
+  forall n P Q R (Qn: environ -> Prop),
+    nth_error Q n = Some Qn ->
+    PROPx P (LOCALx Q (SEPx R)) |-- local Qn.
+Proof.
+intros.
+apply andp_left2. apply andp_left1.
+go_lowerx. normalize.
+revert Q H H0; induction n; destruct Q; intros; inv H.
+destruct H0; auto.
+destruct H0. apply (IHn Q); auto.
+Qed.
+
+(* Hint Rewrite move_prop_from_SEP move_local_from_SEP : norm. *)
+
+Lemma lower_PROP_LOCAL_SEP:
+  forall P Q R rho, PROPx P (LOCALx Q (SEPx R)) rho = 
+     (!!fold_right and True P && (local (fold_right (`and) (`True) Q) && (fold_right sepcon emp R))) rho.
+Proof. reflexivity. Qed.
+Hint Rewrite lower_PROP_LOCAL_SEP : norm.
+
+Lemma lower_TT: forall rho, @TT (environ->mpred) _ rho = @TT mpred Nveric.
+Proof. reflexivity. Qed.
+Hint Rewrite lower_TT : norm.
+
+Lemma lower_FF: forall rho, @FF (environ->mpred) _ rho = @FF mpred Nveric.
+Proof. reflexivity. Qed.
+Hint Rewrite lower_FF : norm.
+
+Lemma remember_value:
+  forall e Espec Delta P Q R c Post,
+  (forall x:val, 
+   @semax Espec Delta (PROPx P (LOCALx (`(eq x) e:: Q) (SEPx R))) c Post) ->
+  @semax Espec Delta (PROPx P (LOCALx Q (SEPx R))) c Post.
+Proof.
+ intros.
+ apply semax_pre0 with (EX x:val, PROPx P (LOCALx (`(eq x) e::Q) (SEPx R))).
+ intro rho. simpl. apply exp_right with (e rho).
+ unfold PROPx, LOCALx; simpl; apply andp_derives; auto.
+ apply andp_derives; auto.
+ unfold local; super_unfold_lift; simpl.
+ apply prop_left; intro. apply prop_right. split; auto.
+ apply extract_exists_pre.  apply H.
+Qed.
+
+Lemma assert_PROP:
+ forall P1 Espec Delta P Q R c Post,
+    PROPx P (LOCALx (tc_environ Delta :: Q) (SEPx R)) |-- !! P1 ->
+   (P1 -> @semax Espec Delta (PROPx P (LOCALx Q (SEPx R))) c Post) ->
+   @semax Espec Delta (PROPx P (LOCALx Q (SEPx R))) c Post.
+Proof.
+intros.
+eapply semax_pre.
+apply andp_right.
+apply H.
+rewrite <- insert_local.
+apply andp_left2; apply derives_refl.
+apply semax_extract_prop.
+auto.
+Qed.
+
+Ltac assert_PROP A :=
+ apply (assert_PROP A); [ | intro].
+
+Lemma assert_LOCAL:
+ forall Q1 Espec Delta P Q R c Post,
+    PROPx P (LOCALx (tc_environ Delta :: Q) (SEPx R)) |-- local Q1 ->
+   @semax Espec Delta (PROPx P (LOCALx (Q1::Q) (SEPx R))) c Post ->
+   @semax Espec Delta (PROPx P (LOCALx Q (SEPx R))) c Post.
+Proof.
+intros.
+eapply semax_pre; try apply H0.
+rewrite <- (insert_local Q1); apply andp_right; auto.
+rewrite <- insert_local; apply andp_left2; auto.
+Qed.
+
+Ltac assert_LOCAL A :=
+ apply (assert_LOCAL A).
+
+Lemma drop_LOCAL':
+  forall (n: nat)  P Q R Post,
+   PROPx P (LOCALx (delete_nth n Q) (SEPx R)) |-- Post ->
+   PROPx P (LOCALx Q (SEPx R)) |-- Post.
+Proof.
+intros.
+eapply derives_trans; try apply H.
+apply andp_derives; auto.
+apply andp_derives; auto.
+intro rho; unfold local, lift1; unfold_lift. apply prop_derives; simpl.
+clear.
+revert Q; induction n; destruct Q; simpl; intros; intuition.
+Qed.
+
+Lemma drop_LOCAL:
+  forall (n: nat) Espec Delta P Q R c Post,
+   @semax Espec Delta (PROPx P (LOCALx (delete_nth n Q) (SEPx R))) c Post ->
+   @semax Espec Delta (PROPx P (LOCALx Q (SEPx R))) c Post.
+Proof.
+intros.
+eapply semax_pre; try apply H.
+rewrite <- insert_local. apply andp_left2.
+apply andp_derives; auto.
+apply andp_derives; auto.
+intro rho; unfold local, lift1; unfold_lift. apply prop_derives; simpl.
+clear.
+revert Q; induction n; destruct Q; simpl; intros; intuition.
+Qed.
+
+Ltac drop_LOCAL n :=
+   first [apply (drop_LOCAL n) | apply (drop_LOCAL' n)];
+    unfold delete_nth.
+
+(**** New experiments regarding TEMP and VAR *)
+
+Definition temp (i: ident) (v: val) : environ -> Prop :=
+   `(eq v) (eval_id i).
+
+Definition var (i: ident) (t: type) (v: val) : environ -> Prop :=
+   `(eq v) (eval_var i t).
+
+
+
+
+
+
+
+
+
+
+
