progs/verif_nest3.v
@@ -8,12 +8,11 @@ Definition get_spec :=
   WITH v : reptype' t_struct_c, p: val
   PRE  [] 
         PROP  ()
-        LOCAL (`(eq p) (eval_var _p t_struct_c))
+        LOCAL (var _p t_struct_c p)
         SEP   (`(data_at Ews t_struct_c (repinj _ v) p))
   POST [ tint ]
         PROP  ()
-        LOCAL (`(eq p) (eval_var _p t_struct_c); 
-               `(eq (Vint (snd (snd (snd v))))) (eval_id 1%positive))
+        LOCAL (var _p t_struct_c p; temp 1%positive (Vint (snd (snd (snd v)))))
         SEP   (`(data_at Ews t_struct_c (repinj _ v) p)).
 
 Definition update222 (i: int) (v: reptype' t_struct_c) : reptype' t_struct_c :=
@@ -24,8 +23,7 @@ Definition set_spec :=
   WITH i : int, v : reptype' t_struct_c, p : val
   PRE  [ _i OF tint ] 
         PROP ()
-        LOCAL(`(eq (Vint i)) (eval_id _i);
-              `(eq p) (eval_var _p t_struct_c))
+        LOCAL(temp _i (Vint i); var _p t_struct_c p)
         SEP(`(data_at Ews t_struct_c (repinj _ v) p))
   POST [ tvoid ]
         `(data_at Ews t_struct_c (repinj _ (update222 i v)) p).
@@ -36,7 +34,7 @@ Definition get_spec2 :=
   WITH v : reptype' t_struct_c, p: val
   PRE  [] 
         PROP  ()
-        LOCAL (`(eq p) (eval_var _p t_struct_c))
+        LOCAL (var _p t_struct_c p)
         SEP   (`(data_at Ews t_struct_c (repinj _ v)) (eval_var _p t_struct_c))
   POST [ tint ]
         PROP  ()
@@ -60,7 +58,7 @@ Definition set_spec2 :=
  DECLARE _set
   WITH i : int, v : reptype' t_struct_c
   PRE  [ _i OF tint ] 
-         PROP () LOCAL(`(eq (Vint i)) (eval_id _i))
+         PROP () LOCAL(temp _i (Vint i))
         SEP(`(data_at Ews t_struct_c (repinj _ v)) (eval_var _p t_struct_c))
   POST [ tvoid ]
         `(data_at Ews t_struct_c (repinj _ (update222 i v))) (eval_var _p t_struct_c).
